add theorem and definitions in H spec list; start proof

HMAC_spec_harvard_list.v
@@ -20,11 +20,11 @@ Notation "f @ g" := (compose f g) (at level 80, right associativity).
 Definition splitVector {A : Type} (h : nat) (t : nat) (l : list A) : (list A * list A) :=
   (firstn h l, skipn t l).
 
-(* 
-Definition mkArg (key:list byte) (pad:byte): list byte := 
+(*
+Definition mkArg (key:list byte) (pad:byte): list byte :=
        (map (fun p => Byte.xor (fst p) (snd p))
           (combine key (sixtyfour pad))).
-Definition mkArgZ key (pad:byte): list Z := 
+Definition mkArgZ key (pad:byte): list Z :=
      map Byte.unsigned (mkArg key pad). *)
 
 (* TODO: length proofs (length xs = length ys) *)
@@ -79,7 +79,7 @@ Section HMAC.
     let (k_Out, k_In) := splitVector c c k in
     h k_Out (h_star_pad k_In m). (* could take head of list *)
 
-  Check GNMAC. 
+  Check GNMAC.
   (*  list bool -> list Blist -> Blist *)
   Check h.
   (* Blist -> Blist -> Blist *)
@@ -110,9 +110,13 @@ Definition GHMAC (k : Blist) :=
 Definition HMAC (k : Blist) :=
   HMAC_2K (BLxor k opad ++ BLxor k ipad).
 
-Check HMAC.                   
+Check HMAC.
 
 End HMAC.
+
+(* --------------------------------- *)
+
+Module Equiv.
 
 Check HMAC.
 
@@ -123,4 +127,81 @@ Check HMAC.
        Blist ->
        (Blist -> list Blist) -> Blist -> Blist -> Blist -> Blist -> Blist *)
 
+(*
+Definition c:nat := (SHA256_.DigestLength * 8)%nat.
+Definition p:=(32 * 8)%nat.
 
+Parameter sha_iv : Bvector (SHA256_.DigestLength * 8).
+Parameter sha_h : Bvector c -> Bvector (c + p) -> Bvector c.
+Parameter sha_splitandpad_vector :
+  Blist -> list (Bvector (SHA256_.DigestLength * 8 + p)).
+
+(* Parameter fpad : Bvector p. *)
+*)
+
+(* TODO does HMAC still need these params? *)
+Definition c:nat := (SHA256_.DigestLength * 8)%nat.
+Definition p:=(32 * 8)%nat.
+
+Parameter sha_iv : Blist.
+Parameter sha_h : Blist -> Blist -> Blist.
+Parameter sha_splitandpad : Blist -> list Blist.
+
+(* -------------- *)
+
+Definition asZ (x : bool) : Z := if x then 1 else 0.
+
+Definition convertByteBits (bits : Blist) (byte : Z) : Prop :=
+  exists (b0 b1 b2 b3 b4 b5 b6 b7 : bool),
+   bits = [b0; b1; b2; b3; b4; b5; b6; b7] /\
+   byte =  (1 * (asZ b0) + 2 * (asZ b1) + 4 * (asZ b2) + 8 * (asZ b3)
+         + 16 * (asZ b4) + 32 * (asZ b5) + 64 * (asZ b6) + 128 * (asZ b7)).
+
+Inductive bytes_bits_lists : Blist -> list Z -> Prop :=
+  | eq_empty : bytes_bits_lists nil nil
+  | eq_cons : forall (bits : Blist) (bytes : list Z)
+                     (b0 b1 b2 b3 b4 b5 b6 b7 : bool) (byte : Z),
+                bytes_bits_lists bits bytes ->
+                convertByteBits [b0; b1; b2; b3; b4; b5; b6; b7] byte ->
+                bytes_bits_lists (b0 :: b1 :: b2 :: b3 :: b4 :: b5 :: b6 :: b7 :: bits)
+                                 (byte :: bytes).
+
+Definition byte_to_64list (byte : byte) : list Z :=
+   map Byte.unsigned (HMAC_SHA256.sixtyfour byte).
+
+(* -------- *)
+
+Theorem HMAC_spec_equiv : forall
+                            (K M H : list Z) (OP IP : byte)
+                            (k m h : Blist) (op ip : Blist),
+  ((length k) * 8)%nat = (c + p)%nat ->
+  (* TODO: might need more hypotheses about lengths *)
+  bytes_bits_lists k K ->
+  bytes_bits_lists m M ->
+  bytes_bits_lists op (byte_to_64list OP) ->
+  bytes_bits_lists ip (byte_to_64list IP) ->
+  HMAC c p sha_h sha_iv sha_splitandpad op ip k m = h ->
+  HMAC_SHA256.HMAC IP OP M K = H ->
+  bytes_bits_lists h H.
+Proof.
+  intros K M H OP IP k m h op ip.
+  intros padded_key_len padded_keys_eq msgs_eq ops_eq ips_eq.
+  intros HMAC_abstract HMAC_concrete.
+
+  intros.
+  unfold p, c in *.
+  simpl in *.
+
+  unfold HMAC in *. simpl in *.
+  unfold HMAC_SHA256.HMAC in *.
+
+  rewrite <- HMAC_abstract. rewrite <- HMAC_concrete.
+
+  induction msgs_eq.
+
+  (* [], [] *)
+  - simpl.
+    (* need to prove that m = [] -> HMAC _ ... _ = [] *)
+    admit.
+
+  - 
